Reduce Resource Usage for UniformPowerOfTwo correctness (#52)
* wip

* Remove another split_on_every_assert

* Simplify full correctness proof

* Add guideline not to split assertions

src/Distributions/UniformPowerOfTwo/Correctness.dfy
@@ -27,6 +27,7 @@ module UniformPowerOfTwoCorrectness {
   ************/
 
   // Definition 50
+  // An approximately uniform sampler: may have too much mass on 0.
   function ProbUniformCut(t: nat, n: nat): Hurd<nat>
     requires n > 0
   {
@@ -91,20 +92,13 @@ module UniformPowerOfTwoCorrectness {
   }
 
   // Equation (4.8)
-  lemma {:vcs_split_on_every_assert} UnifCorrectness(n: nat, k: nat)
+  lemma UnifCorrectness(n: nat, k: nat)
     requires (n == 0 && k == 0) || (k != 0 && Power(2, k - 1) <= n < Power(2, k))
     ensures forall m: nat :: UnifIsCorrect(n, k, m)
   {
     forall m: nat ensures UnifIsCorrect(n, k, m) {
       if (n == 0 && k == 0) {
-        assert Power(2, k) == 1;
-        if m == 0 {
-          assert (iset s | ProbUnif(n)(s).0 == m) == (iset s {:trigger true} | true);
-          RNGHasMeasure();
-        } else {
-          assert (iset s | ProbUnif(n)(s).0 == m) == iset{};
-          RNGHasMeasure();
-        }
+        UnifCorrectnessCaseNZeroKZero(m);
       } else {
         assert (k != 0 && Power(2, k - 1) <= n < Power(2, k));
         assert n > 0;
@@ -117,155 +111,213 @@ module UniformPowerOfTwoCorrectness {
           assert n == 1;
           assert n / 2 == 0;
           if m % 2 == 0 {
-            calc {
-              mu(iset s | ProbUnif(n)(s).0 == m);
-            == { ProbUnifCaseSplit(n, m); }
-              mu(iset s | 2*ProbUnif(n / 2)(s).0 == m) / 2.0;
-            == { assert (iset s | 2*ProbUnif(n / 2)(s).0 == m) == (iset s {:trigger 0 == m} | 0 == m); }
-              mu(iset s {:trigger 0 == m} | 0 == m) / 2.0;
-            }
-            if m < Power(2, k) {
-              assert m == 0;
-              calc {
-                mu(iset s | ProbUnif(n)(s).0 == m);
-              ==
-                mu(iset s {:trigger 0 == m} | 0 == m) / 2.0;
-              == { assert (iset s: RNG {:trigger 0 == m} | 0 == m) == (iset s {:trigger true} | true); }
-                mu(iset s {:trigger true} | true) / 2.0;
-              == { RNGHasMeasure(); }
-                1.0 / 2.0;
-              == { assert 2.0 == 2 as real; DivisionSubstitute(1.0, 2.0, 2 as real); }
-                1.0 / (2 as real);
-              == { assert k == 1; assert Power(2, k) == 2; assert Power(2, k) as real == 2 as real; DivisionSubstitute(1.0, 2 as real, Power(2, k) as real); }
-                1.0 / (Power(2, k) as real);
-              }
-            } else {
-              assert m != 0;
-              calc {
-                mu(iset s | ProbUnif(n)(s).0 == m);
-              ==
-                mu(iset s {:trigger 0 == m} | 0 == m) / 2.0;
-              == { assert (iset s: RNG {:trigger 0 == m} | 0 == m) == iset{}; }
-                mu(iset {}) / 2.0;
-              == { RNGHasMeasure(); }
-                0.0 / 2.0;
-              ==
-                0.0;
-              }
-            }
+            UnifCorrectnessCaseKOneMEven(n, m);
           } else {
             assert m % 2 == 1;
-            calc {
-              mu(iset s | ProbUnif(n)(s).0 == m);
-            == { ProbUnifCaseSplit(n, m); }
-              mu(iset s | 2*ProbUnif(n / 2)(s).0 + 1 == m) / 2.0;
-            == { assert (iset s | 2*ProbUnif(n / 2)(s).0 + 1 == m) == (iset s {:trigger 1 == m} | 1 == m); }
-              mu(iset s {:trigger 1 == m} | 1 == m) / 2.0;
-            }
-            if m < Power(2, k) {
-              assert m == 1;
-              calc {
-                mu(iset s | ProbUnif(n)(s).0 == m);
-              ==
-                mu(iset s {:trigger 1 == m} | 1 == m) / 2.0;
-              == { assert (iset s: RNG {:trigger 1 == m} | 1 == m) == (iset s {:trigger true} | true); }
-                mu(iset s {:trigger true} | true) / 2.0;
-              == { RNGHasMeasure(); DivisionSubstituteAlternativeReal(2.0, mu(iset s {:trigger true} | true), 1.0); }
-                1.0 / 2.0;
-              == { assert k == 1; assert 2.0 == 2 as real == Power(2, k) as real; DivisionSubstitute(1.0, 2.0, Power(2, k) as real); }
-                1.0 / (Power(2, k) as real);
-              }
-            } else {
-              assert m != 1;
-              calc {
-                mu(iset s: RNG | ProbUnif(n)(s).0 == m);
-              ==
-                mu(iset s: RNG {:trigger 1 == m} | 1 == m) / 2.0;
-              == { assert (iset s: RNG {:trigger 1 == m} | 1 == m) == iset{}; }
-                mu(iset {}) / 2.0;
-              == { RNGHasMeasure(); }
-                0.0 / 2.0;
-              ==
-                0.0;
-              }
-            }
+            UnifCorrectnessCaseKOneMOdd(n, m);
           }
         } else {
           assert Power(2, k - 1) / 2 <= n / 2 < Power(2, k) / 2;
           assert Power(2, k - 2) <= n / 2 < Power(2, k - 1);
-
           var u := m / 2;
           if m % 2 == 0 {
-            assert m == 2 * u;
-            calc {
-              mu(iset s | ProbUnif(n)(s).0 == m);
-            == { ProbUnifCaseSplit(n, m); }
-              mu(iset s | 2 * ProbUnif(n / 2)(s).0 == m) / 2.0;
-            == { assert (iset s | 2 * ProbUnif(n / 2)(s).0 == m) == (iset s | ProbUnif(n / 2)(s).0 == u); }
-              mu(iset s | ProbUnif(n / 2)(s).0 == u) / 2.0;
-            }
-            if m < Power(2, k) {
-              assert mu(iset s | ProbUnif(n / 2)(s).0 == u) == 1.0 / (Power(2, k - 1) as real) by {
-                assert u < Power(2, k - 1);
-                UnifCorrectness(n / 2, k - 1);
-                assert UnifIsCorrect(n / 2, k - 1, u);
-              }
-              calc {
-                mu(iset s | ProbUnif(n)(s).0 == m);
-              ==
-                mu(iset s | ProbUnif(n / 2)(s).0 == u) / 2.0;
-              ==
-                (1.0 / Power(2, k - 1) as real) / 2.0;
-              ==
-                1.0 / (Power(2, k - 1) as real * 2.0);
-              ==
-                1.0 / (Power(2, k - 1) * 2) as real;
-              ==
-                1.0 / (Power(2, k) as real);
-              }
-            } else {
-              assert u >= Power(2, k - 1);
-              UnifCorrectness(n / 2, k - 1);
-              assert UnifIsCorrect(n / 2, k - 1, u);
-              assert mu(iset s | ProbUnif(n)(s).0 == m) == 0.0;
-            }
+            UnifCorrectnessCaseKGreaterOneMEven(n, k, m);
           } else {
-            assert m == 2 * u + 1;
-            calc {
-              mu(iset s | ProbUnif(n)(s).0 == m);
-            == { ProbUnifCaseSplit(n, m); }
-              mu(iset s | 2 * ProbUnif(n / 2)(s).0 + 1 == m) / 2.0;
-            == { assert (iset s | 2 * ProbUnif(n / 2)(s).0 + 1 == m) == (iset s | ProbUnif(n / 2)(s).0 == u); }
-              mu(iset s | ProbUnif(n / 2)(s).0 == u) / 2.0;
-            }
-            if m < Power(2, k) {
-              assert mu(iset s | ProbUnif(n / 2)(s).0 == u) == 1.0 / (Power(2, k - 1) as real) by {
-                assert u < Power(2, k - 1);
-                UnifCorrectness(n / 2, k - 1);
-                assert UnifIsCorrect(n / 2, k - 1, u);
-              }
-              calc {
-                mu(iset s | ProbUnif(n)(s).0 == m);
-              ==
-                mu(iset s | ProbUnif(n / 2)(s).0 == u) / 2.0;
-              ==
-                (1.0 / Power(2, k - 1) as real) / 2.0;
-              ==
-                1.0 / (Power(2, k - 1) as real * 2.0);
-              ==
-                1.0 / (Power(2, k - 1) * 2) as real;
-              ==
-                1.0 / (Power(2, k) as real);
-              }
-            } else {
-              assert u >= Power(2, k - 1);
-              UnifCorrectness(n / 2, k - 1);
-              assert UnifIsCorrect(n / 2, k - 1, u);
-              assert mu(iset s | ProbUnif(n)(s).0 == m) == 0.0;
-            }
+            UnifCorrectnessCaseKGreaterOneMOdd(n, k, m);
           }
         }
       }
+    }
+  }
+
+  lemma UnifCorrectnessCaseNZeroKZero(m: nat)
+    ensures UnifIsCorrect(0, 0, m)
+  {
+    assert Power(2, 0) == 1;
+    if m == 0 {
+      assert (iset s | ProbUnif(0)(s).0 == m) == (iset s {:trigger true} | true);
+      RNGHasMeasure();
+    } else {
+      assert (iset s | ProbUnif(0)(s).0 == m) == iset{};
+      RNGHasMeasure();
+    }
+  }
+
+  lemma UnifCorrectnessCaseKOneMEven(n: nat, m: nat)
+    requires 1 <= n < 2
+    requires m % 2 == 0
+    ensures UnifIsCorrect(n, 1, m)
+  {
+    calc {
+      mu(iset s | ProbUnif(n)(s).0 == m);
+    == { ProbUnifCaseSplit(n, m); }
+      mu(iset s | 2*ProbUnif(n / 2)(s).0 == m) / 2.0;
+    == { assert (iset s | 2*ProbUnif(n / 2)(s).0 == m) == (iset s {:trigger 0 == m} | 0 == m); }
+      mu(iset s {:trigger 0 == m} | 0 == m) / 2.0;
+    }
+    if m < Power(2, 1) {
+      assert m == 0;
+      calc {
+        mu(iset s | ProbUnif(n)(s).0 == m);
+      ==
+        mu(iset s {:trigger 0 == m} | 0 == m) / 2.0;
+      == { assert (iset s: RNG {:trigger 0 == m} | 0 == m) == (iset s {:trigger true} | true); }
+        mu(iset s {:trigger true} | true) / 2.0;
+      == { RNGHasMeasure(); }
+        1.0 / 2.0;
+      ==
+        1.0 / (2 as real);
+      == { assert Power(2, 1) == 2; }
+        1.0 / (Power(2, 1) as real);
+      }
+    } else {
+      assert m != 0;
+      calc {
+        mu(iset s | ProbUnif(n)(s).0 == m);
+      ==
+        mu(iset s {:trigger 0 == m} | 0 == m) / 2.0;
+      == { assert (iset s: RNG {:trigger 0 == m} | 0 == m) == iset{}; }
+        mu(iset {}) / 2.0;
+      == { RNGHasMeasure(); }
+        0.0 / 2.0;
+      ==
+        0.0;
+      }
+    }
+  }
+
+  lemma UnifCorrectnessCaseKOneMOdd(n: nat, m: nat)
+    requires 1 <= n < 2
+    requires m % 2 == 1
+    ensures UnifIsCorrect(n, 1, m)
+  {
+    calc {
+        mu(iset s | ProbUnif(n)(s).0 == m);
+      == { ProbUnifCaseSplit(n, m); }
+        mu(iset s | 2*ProbUnif(n / 2)(s).0 + 1 == m) / 2.0;
+      == { assert (iset s | 2*ProbUnif(n / 2)(s).0 + 1 == m) == (iset s {:trigger 1 == m} | 1 == m); }
+        mu(iset s {:trigger 1 == m} | 1 == m) / 2.0;
+      }
+      if m < Power(2, 1) {
+        assert m == 1;
+        calc {
+          mu(iset s | ProbUnif(n)(s).0 == m);
+        ==
+          mu(iset s {:trigger 1 == m} | 1 == m) / 2.0;
+        == { assert (iset s: RNG {:trigger 1 == m} | 1 == m) == (iset s {:trigger true} | true); }
+          mu(iset s {:trigger true} | true) / 2.0;
+        == { RNGHasMeasure(); DivisionSubstituteAlternativeReal(2.0, mu(iset s {:trigger true} | true), 1.0); }
+          1.0 / 2.0;
+        ==
+          1.0 / (Power(2, 1) as real);
+        }
+      } else {
+        assert m != 1;
+        calc {
+          mu(iset s: RNG | ProbUnif(n)(s).0 == m);
+        ==
+          mu(iset s: RNG {:trigger 1 == m} | 1 == m) / 2.0;
+        == { assert (iset s: RNG {:trigger 1 == m} | 1 == m) == iset{}; }
+          mu(iset {}) / 2.0;
+        == { RNGHasMeasure(); }
+          0.0 / 2.0;
+        ==
+          0.0;
+        }
+    }
+  }
+
+  lemma UnifCorrectnessCaseKGreaterOneMEven(n: nat, k: nat, m: nat)
+    requires k >= 2
+    requires Power(2, k - 1) <= n < Power(2, k)
+    requires m % 2 == 0
+    ensures UnifIsCorrect(n, k, m)
+  {
+    var u := m / 2;
+    assert m == 2 * u;
+    calc {
+      mu(iset s | ProbUnif(n)(s).0 == m);
+    == { ProbUnifCaseSplit(n, m); }
+      mu(iset s | 2 * ProbUnif(n / 2)(s).0 == m) / 2.0;
+    == { assert (iset s | 2 * ProbUnif(n / 2)(s).0 == m) == (iset s | ProbUnif(n / 2)(s).0 == u); }
+      mu(iset s | ProbUnif(n / 2)(s).0 == u) / 2.0;
+    }
+    if m < Power(2, k) {
+      assert mu(iset s | ProbUnif(n / 2)(s).0 == u) == 1.0 / (Power(2, k - 1) as real) by {
+        assert u < Power(2, k - 1);
+        UnifCorrectness(n / 2, k - 1);
+        assert UnifIsCorrect(n / 2, k - 1, u);
+      }
+      calc {
+        mu(iset s | ProbUnif(n)(s).0 == m);
+      ==
+        mu(iset s | ProbUnif(n / 2)(s).0 == u) / 2.0;
+      ==
+        (1.0 / Power(2, k - 1) as real) / 2.0;
+      == { PowerOfTwoLemma(k - 1); }
+        1.0 / (Power(2, k) as real);
+      }
+      assert UnifIsCorrect(n / 2, k - 1, u);
+    } else {
+      assert u >= Power(2, k - 1);
+      UnifCorrectness(n / 2, k - 1);
+      assert UnifIsCorrect(n / 2, k - 1, u);
+      assert mu(iset s | ProbUnif(n)(s).0 == m) == 0.0;
+      assert UnifIsCorrect(n / 2, k - 1, u);
+    }
+  }
+
+  lemma UnifCorrectnessCaseKGreaterOneMOdd(n: nat, k: nat, m: nat)
+    requires k >= 2
+    requires Power(2, k - 1) <= n < Power(2, k)
+    requires m % 2 == 1
+    ensures UnifIsCorrect(n, k, m)
+  {
+    var u := m / 2;
+    assert m == 2 * u + 1;
+    calc {
+      mu(iset s | ProbUnif(n)(s).0 == m);
+    == { ProbUnifCaseSplit(n, m); }
+      mu(iset s | 2 * ProbUnif(n / 2)(s).0 + 1 == m) / 2.0;
+    == { assert (iset s | 2 * ProbUnif(n / 2)(s).0 + 1 == m) == (iset s | ProbUnif(n / 2)(s).0 == u); }
+      mu(iset s | ProbUnif(n / 2)(s).0 == u) / 2.0;
+    }
+    if m < Power(2, k) {
+      assert mu(iset s | ProbUnif(n / 2)(s).0 == u) == 1.0 / (Power(2, k - 1) as real) by {
+        assert u < Power(2, k - 1);
+        UnifCorrectness(n / 2, k - 1);
+        assert UnifIsCorrect(n / 2, k - 1, u);
+      }
+      calc {
+        mu(iset s | ProbUnif(n)(s).0 == m);
+      ==
+        mu(iset s | ProbUnif(n / 2)(s).0 == u) / 2.0;
+      ==
+        (1.0 / Power(2, k - 1) as real) / 2.0;
+      == { PowerOfTwoLemma(k - 1); }
+        1.0 / (Power(2, k) as real);
+      }
+      assert UnifIsCorrect(n, k, m);
+    } else {
+      assert u >= Power(2, k - 1);
+      UnifCorrectness(n / 2, k - 1);
+      assert UnifIsCorrect(n / 2, k - 1, u);
+      assert mu(iset s | ProbUnif(n)(s).0 == m) == 0.0;
+      assert UnifIsCorrect(n, k, m);
+    }
+  }
+
+  lemma PowerOfTwoLemma(k: nat)
+    ensures (1.0 / Power(2, k) as real) / 2.0 == 1.0 / (Power(2, k + 1) as real)
+  {
+    calc {
+      (1.0 / Power(2, k) as real) / 2.0;
+      == { DivDivToDivMul(1.0, Power(2, k) as real, 2.0); }
+        1.0 / (Power(2, k) as real * 2.0);
+      == { NatMulNatToReal(Power(2, k), 2); }
+        1.0 / (Power(2, k) * 2) as real;
+      ==
+        1.0 / (Power(2, k + 1) as real);
     }
   }
 
@@ -280,31 +332,27 @@ module UniformPowerOfTwoCorrectness {
       var p := (s: RNG) => ProbUnif(n-1)(s).0 < n;
       ForAllStar(p)
 
-  lemma {:vcs_split_on_every_assert} ProbUnifIsMeasurePreserving(n: nat)
-    ensures
-      var f := (s: RNG) => ProbUnif(n)(s).1;
-      IsMeasurePreserving(event_space, mu, event_space, mu, f)
+  function ProbUnif1(n: nat): RNG -> RNG {
+    (s: RNG) => ProbUnif(n)(s).1
+  }
+
+  lemma ProbUnifIsMeasurePreserving(n: nat)
+    ensures IsMeasurePreserving(event_space, mu, event_space, mu, ProbUnif1(n))
   {
-    var f := (s: RNG) => ProbUnif(n)(s).1;
+    var f := ProbUnif1(n);
     assert IsMeasurable(event_space, event_space, f) by {
       ProbUnifIsIndepFn(n);
       assert IsIndepFn(ProbUnif(n));
     }
-    var g := (s: RNG) => ProbUnif(n / 2)(s).1;
+    var g := ProbUnif1(n / 2);
     if n == 0 {
       forall e | e in event_space ensures mu(PreImage(f, e)) == mu(e) {
-        calc {
-          mu(PreImage(f, e));
-        == { assert PreImage(f, e) == (iset s | f(s) in e); }
-          mu(iset s | f(s) in e);
-        == { assert (iset s | f(s) in e) == (iset s | ProbUnif(n)(s).1 in e); }
-          mu(iset s | ProbUnif(n)(s).1 in e);
-        == { assert (iset s | ProbUnif(n)(s).1 in e) == (iset s | s in e); }
-          mu(iset s | s in e);
-        == { assert (iset s | s in e) == e; }
-          mu(e);
+        forall s: RNG ensures f(s) == s {
+          assert f(s) == s;
         }
+        PreImageIdentity(f, e);
       }
+      assert IsMeasurePreserving(event_space, mu, event_space, mu, f);
     } else {
       forall e | e in event_space ensures mu(PreImage(f, e)) == mu(e) {
         var e' := (iset s | Tail(s) in e);
@@ -313,43 +361,39 @@ module UniformPowerOfTwoCorrectness {
           TailIsMeasurePreserving();
           assert IsMeasurable(event_space, event_space, Tail);
         }
-        assert A: forall s :: ProbUnif(n)(s).1 in e <==> Tail(ProbUnif(n / 2)(s).1) in e by {
-          forall s ensures ProbUnif(n)(s).1 in e <==> Tail(ProbUnif(n / 2)(s).1) in e {
-            ProbUnifTailDecompose(n, s);
+        assert PreImage(f, e) == PreImage(g, e') by {
+          assert forall s :: f(s) in e <==> g(s) in e' by {
+            forall s ensures f(s) in e <==> g(s) in e' {
+              calc {
+                f(s) in e;
+                <==> { assert f(s) == ProbUnif(n)(s).1; }
+                ProbUnif(n)(s).1 in e;
+                <==> { ProbUnifTailDecompose(n, s); }
+                Tail(ProbUnif(n / 2)(s).1) in e;
+                <==>
+                ProbUnif(n / 2)(s).1 in e';
+                <==> { assert ProbUnif(n / 2)(s).1 == g(s); }
+                g(s) in e';
+              }
+            }
           }
+          PreImagesEqual(f, e, g, e');
         }
-        assert B: forall s :: Tail(ProbUnif(n / 2)(s).1) in e <==> ProbUnif(n / 2)(s).1 in e' by {
-          forall s ensures Tail(ProbUnif(n / 2)(s).1) in e <==> ProbUnif(n / 2)(s).1 in e' {
-            assert Tail(ProbUnif(n / 2)(s).1) in e <==> ProbUnif(n / 2)(s).1 in e';
+        assert mu(PreImage(f, e)) == mu(e) by {
+          calc {
+            mu(PreImage(f, e));
+          ==
+            mu(PreImage(g, e'));
+          == { ProbUnifIsMeasurePreserving(n / 2); assert IsMeasurePreserving(event_space, mu, event_space, mu, g); assert e' in event_space; }
+            mu(e');
+          == { assert e' == PreImage(Tail, e); }
+            mu(PreImage(Tail, e));
+          == { TailIsMeasurePreserving(); }
+            mu(e);
           }
-        }
-        assert C: forall s :: f(s) in e <==> ProbUnif(n)(s).1 in e by {
-          forall s ensures f(s) in e <==> ProbUnif(n)(s).1 in e {
-            assert f(s) == ProbUnif(n)(s).1;
-          }
-        }
-        calc {
-          mu(PreImage(f, e));
-        == { assert PreImage(f, e) == (iset s | f(s) in e); }
-          mu(iset s | f(s) in e);
-        == { assert (iset s | f(s) in e) == (iset s | ProbUnif(n)(s).1 in e) by { reveal C; } }
-          mu(iset s | ProbUnif(n)(s).1 in e);
-        == { assert (iset s | ProbUnif(n)(s).1 in e) == (iset s | Tail(ProbUnif(n / 2)(s).1) in e) by { reveal A; } }
-          mu(iset s | Tail(ProbUnif(n / 2)(s).1) in e);
-        == { assert (iset s | Tail(ProbUnif(n / 2)(s).1) in e) == (iset s | ProbUnif(n / 2)(s).1 in e') by { reveal B; } }
-          mu(iset s | ProbUnif(n / 2)(s).1 in e');
-        == { assert (iset s | ProbUnif(n / 2)(s).1 in e') == (iset s | g(s) in e'); }
-          mu(iset s | g(s) in e');
-        == { assert (iset s | g(s) in e') == PreImage(g, e'); }
-          mu(PreImage(g, e'));
-        == { ProbUnifIsMeasurePreserving(n / 2); assert IsMeasurePreserving(event_space, mu, event_space, mu, g); assert e' in event_space; }
-          mu(e');
-        == { assert e' == PreImage(Tail, e); }
-          mu(PreImage(Tail, e));
-        == { TailIsMeasurePreserving(); }
-          mu(e);
         }
       }
+      assert IsMeasurePreserving(event_space, mu, event_space, mu, f);
     }
   }
 
@@ -357,18 +401,14 @@ module UniformPowerOfTwoCorrectness {
     requires n != 0
     ensures ProbUnif(n)(s).1 == Tail(ProbUnif(n / 2)(s).1)
   {
-    var f := (m: nat) =>
-        var g := (b: bool) =>
-                   Return(if b then 2*m + 1 else 2*m);
-        Bind(Deconstruct, g);
     var (a, s') := ProbUnif(n / 2)(s);
     var (b, s'') := Deconstruct(s');
     calc {
       ProbUnif(n)(s).1;
     ==
-      Bind(ProbUnif(n / 2), f)(s).1;
+      Bind(ProbUnif(n / 2), UnifStep)(s).1;
     ==
-      f(a)(s').1;
+      UnifStep(a)(s').1;
     ==
       Bind(Deconstruct, (b: bool) => Return(if b then 2*a + 1 else 2*a))(s').1;
     ==
@@ -391,18 +431,14 @@ module UniformPowerOfTwoCorrectness {
       <==>
       (b && 2*a + 1 == m) || (!b && 2*a == m)
   {
-    var f := (m: nat) =>
-        var g := (b: bool) =>
-                   Return(if b then 2*m + 1 else 2*m);
-        Bind(Deconstruct, g);
     var (a, s') := ProbUnif(n / 2)(s);
     var (b, s'') := Deconstruct(s');
     calc {
       ProbUnif(n)(s).0;
     ==
-      Bind(ProbUnif(n / 2), f)(s).0;
+      Bind(ProbUnif(n / 2), UnifStep)(s).0;
     ==
-      f(a)(s').0;
+      UnifStep(a)(s').0;
     ==
       Bind(Deconstruct, b => Return(if b then 2*a + 1 else 2*a))(s').0;
     ==
@@ -412,7 +448,7 @@ module UniformPowerOfTwoCorrectness {
     }
   }
 
-  lemma {:vcs_split_on_every_assert} ProbUnifCorrectnessEvenCaseIff(n: nat, s: RNG, m: nat)
+  lemma ProbUnifCorrectnessEvenCaseIff(n: nat, s: RNG, m: nat)
     requires m % 2 == 0
     requires n > 0
     ensures
@@ -420,22 +456,13 @@ module UniformPowerOfTwoCorrectness {
       var b := Deconstruct(ProbUnif(n / 2)(s).1).0;
       ProbUnif(n)(s).0 == m <==> (!b && 2*a == m)
   {
-    var a := ProbUnif(n / 2)(s).0;
+    var a: nat := ProbUnif(n / 2)(s).0;
     var b := Deconstruct(ProbUnif(n / 2)(s).1).0;
     if ProbUnif(n)(s).0 == m {
       if (b && 2*a + 1 == m) {
-        assert A: (2*a + 1) / 2 == 1 by {
-          calc {
-            (2*a + 1) / 2;
-          == { LemmaAboutNatDivision(2*a + 1, 2); }
-            ((2*a + 1) as real / 2 as real).Floor;
-          == { assert (2*a + 1) as real / 2 as real == 1 as real; }
-            (1 as real).Floor;
-          ==
-            1;
-          }
+        assert m % 2 == 1 by {
+          DivModAddMultiple(2, 1, a);
         }
-        assert m % 2 == 1 by { assert m == 2*a + 1; reveal A; assert m / 2 == 1 by { DivisionSubstituteAlternative(2, m, 2*a + 1); } }
         assert m % 2 == 0;
         assert false;
       }
@@ -450,7 +477,7 @@ module UniformPowerOfTwoCorrectness {
     }
   }
 
-  lemma {:vcs_split_on_every_assert} ProbUnifOddCaseIff(n: nat, s: RNG, m: nat)
+  lemma ProbUnifOddCaseIff(n: nat, s: RNG, m: nat)
     requires m % 2 == 1
     requires n > 0
     ensures
@@ -506,7 +533,7 @@ module UniformPowerOfTwoCorrectness {
     }
   }
 
-  lemma {:vcs_split_on_every_assert} ProbUnifEvenCase(n: nat, m: nat)
+  lemma ProbUnifEvenCase(n: nat, m: nat)
     requires m % 2 == 0
     requires n > 0
     ensures mu(iset s | ProbUnif(n)(s).0 == m) == mu(iset s | 2*ProbUnif(n / 2)(s).0 == m) / 2.0
@@ -515,9 +542,9 @@ module UniformPowerOfTwoCorrectness {
     var b_of := (s: RNG) => Deconstruct(ProbUnif(n / 2)(s).1).0;
     var A: iset<nat> := (iset x | 2*x == m);
     var E: iset<RNG> := (iset s | Deconstruct(s).0 == false);
-    var f := (s: RNG) => ProbUnif(n / 2)(s).1;
+    var f := ProbUnif1(n / 2);
 
-    var e1 := (iset s | ProbUnif(n / 2)(s).1 in E);
+    var e1 := (iset s | ProbUnif1(n / 2)(s) in E);
     var e2 := (iset s | ProbUnif(n / 2)(s).0 in A);
 
     assert Eq1: (iset s | !b_of(s)) == e1 by {
@@ -535,24 +562,28 @@ module UniformPowerOfTwoCorrectness {
       }
     }
 
-    assert Eq4: e1 == PreImage(f, E) by {
+    assert Eq4: e1 == PreImage(ProbUnif1(n / 2), E) by {
       forall s ensures ProbUnif(n / 2)(s).1 in E <==> f(s) in E {
       }
     }
 
-    assert E in event_space && mu(E) == 0.5 by {
+    assert EMeasure: E in event_space && mu(E) == 0.5 by {
       assert E == (iset s | Head(s) == false);
       HeadIsMeasurable(false);
     }
 
     assert Indep: mu(e1 * e2) == mu(e1) * mu(e2) by {
+      assert e1 == (iset s | ProbUnif(n / 2)(s).1 in E) by {
+        forall s ensures s in e1 <==> ProbUnif(n / 2)(s).1 in E {
+        }
+      }
       assert AreIndepEvents(event_space, mu, e1, e2) by {
         assert IsIndepFunction(ProbUnif(n / 2)) by {
           assert IsIndepFn(ProbUnif(n / 2)) by {
             ProbUnifIsIndepFn(n / 2);
           }
         }
-        assert E in event_space;
+        assert E in event_space by { reveal EMeasure; }
         assert IsIndepFunctionCondition(ProbUnif(n / 2), A, E);
       }
       AreIndepEventsConjunctElimination(e1, e2);
@@ -561,23 +592,22 @@ module UniformPowerOfTwoCorrectness {
     assert Prob: 0.5 == mu(e1) by {
       calc {
         0.5;
-      ==
+      == { reveal EMeasure; }
         mu(E);
-      == { ProbUnifIsMeasurePreserving(n / 2); }
-        mu(PreImage(f, E));
+      == { reveal EMeasure; ProbUnifIsMeasurePreserving(n / 2); }
+        mu(PreImage(ProbUnif1(n / 2), E));
       == { reveal Eq4; }
         mu(e1);
       }
     }
 
-    var p := (s: RNG) => s in (iset s | !b_of(s) && 2*a_of(s) == m) <==> s in (iset s | !b_of(s)) && s in (iset s | 2*a_of(s) == m);
-
-    assert Inter: forall s :: p(s) by {
+    assert Inter: (iset s | !b_of(s) && 2*a_of(s) == m) == (iset s | !b_of(s)) * (iset s | 2*a_of(s) == m) by {
       forall s ensures !b_of(s) && 2*a_of(s) == m <==> !b_of(s) && 2*a_of(s) == m {
       }
     }
 
     assert MulSub: mu(e1) * mu(e2) == 0.5 * mu(e2) by {
+      reveal EMeasure;
       assert mu(e1) == 0.5 by { reveal Prob; }
       assert mu(e1) == 0.5 ==> mu(e1) * mu(e2) == 0.5 * mu(e2);
     }
@@ -586,7 +616,7 @@ module UniformPowerOfTwoCorrectness {
       mu(iset s | ProbUnif(n)(s).0 == m);
     == { ProbUnifEvenCaseSetEquality(n, m); }
       mu(iset s | !b_of(s) && 2*a_of(s) == m);
-    == { assert (iset s | !b_of(s) && 2*a_of(s) == m) == (iset s | !b_of(s)) * (iset s | 2*a_of(s) == m) by { reveal Inter; } }
+    == {  reveal Inter; }
       mu((iset s | !b_of(s)) * (iset s | 2*a_of(s) == m));
     == { reveal Eq1; reveal Eq2; }
       mu(e1 * e2);
@@ -603,7 +633,7 @@ module UniformPowerOfTwoCorrectness {
     }
   }
 
-  lemma {:vcs_split_on_every_assert} ProbUnifOddCase(n: nat, m: nat)
+  lemma ProbUnifOddCase(n: nat, m: nat)
     requires m % 2 == 1
     requires n > 0
     ensures mu(iset s | ProbUnif(n)(s).0 == m) == mu(iset s | 2*ProbUnif(n / 2)(s).0 + 1 == m) / 2.0
